hyperheap ... removing a couple of fsis

lib/FStar.Map.fst
@@ -3,11 +3,17 @@ open Prims.PURE
 open FStar.Set
 open FStar.FunctionalExtensionality
 
-type t (key:Type) (value:Type) = {
+abstract type t (key:Type) (value:Type) = {
   mappings: key -> Tot value;
   domain:   key -> Tot bool
 }
 
+abstract val sel: t 'key 'value -> 'key -> Tot 'value
+abstract val upd: t 'key 'value -> 'key -> 'value -> Tot (t 'key 'value)
+abstract val const: 'value -> Tot (t 'key 'value)
+abstract val concat: t 'key 'value -> t 'key 'value -> Tot (t 'key 'value)
+abstract val contains: t 'key 'value -> 'key -> Tot bool
+abstract val restrict: set 'key -> t 'key 'value -> Tot (t 'key 'value)
 
 let sel m k = m.mappings k
 let upd m k v = {
@@ -28,6 +34,51 @@ let restrict s m = {
   domain =   (fun x -> mem x s && contains m x)
 }
 
+abstract val lemma_SelUpd1: m:t 'key 'value -> k:'key -> v:'value ->
+                   Lemma (requires True) (ensures (sel (upd m k v) k = v))
+		   [SMTPat (sel (upd m k v) k)]
+
+abstract val lemma_SelUpd2: m:t 'key 'value -> k1:'key -> k2:'key -> v:'value ->
+                   Lemma (requires True) (ensures (k2=!=k1 ==> sel (upd m k2 v) k1 = sel m k1))
+                   [SMTPat (sel (upd m k2 v) k1)]
+
+abstract val lemma_SelConst: v:'value -> k:'key ->
+                    Lemma (requires True) (ensures (sel (const v) k == v))
+                    [SMTPat (sel (const v) k)]
+
+abstract val lemma_SelRestrict: m:t 'key 'value -> ks:set 'key -> k:'key ->
+                       Lemma (requires True) (ensures (mem k ks ==> sel (restrict ks m) k == sel m k))
+                       [SMTPat (sel (restrict ks m) k)]
+
+abstract val lemma_SelConcat1: m1:t 'key 'value -> m2:t 'key 'value -> k:'key ->
+                      Lemma (requires True) (ensures (contains m2 k ==> sel (concat m1 m2) k==sel m2 k))
+                      [SMTPat (sel (concat m1 m2) k)]
+
+abstract val lemma_SelConcat2: m1:t 'key 'value -> m2:t 'key 'value -> k:'key ->
+                      Lemma (requires True) (ensures (not(contains m2 k) ==> sel (concat m1 m2) k==sel m1 k))
+                      [SMTPat (sel (concat m1 m2) k)]
+
+abstract val lemma_InDomUpd1: m:t 'key 'value -> k1:'key -> k2:'key -> v:'value ->
+                     Lemma (requires True) (ensures (contains (upd m k1 v) k2 == (k1=k2 || contains m k2)))
+                     [SMTPat (contains (upd m k1 v) k2)]
+
+abstract val lemma_InDomUpd2: m:t 'key 'value -> k1:'key -> k2:'key -> v:'value ->
+                     Lemma (requires True) (ensures (k2=!=k1 ==> contains (upd m k2 v) k1 == contains m k1))
+                     [SMTPat (contains (upd m k2 v) k1)]
+
+abstract val lemma_InDomConstMap: v:'value -> k:'key ->
+                         Lemma (requires True) (ensures (contains (const v) k))
+                         [SMTPat (contains (const v) k)]
+
+abstract val lemma_InDomConcat: m1:t 'key 'value -> m2:t 'key 'value -> k:'key ->
+                 Lemma (requires True) (ensures (contains (concat m1 m2) k==(contains m1 k || contains m2 k)))
+                 [SMTPat (contains (concat m1 m2) k)]
+
+abstract val lemma_InDomRestrict: m:t 'key 'value -> ks:set 'key -> k:'key ->
+                         Lemma (requires True) (ensures (contains (restrict ks m) k == (mem k ks && contains m k)))
+                         [SMTPat (contains (restrict ks m) k)]
+
+
 let lemma_SelUpd1 m k v        = ()
 let lemma_SelUpd2 m k1 k2 v    = ()
 let lemma_SelConst v k         = ()
@@ -40,13 +91,33 @@ let lemma_InDomConstMap v k    = ()
 let lemma_InDomConcat m1 m2 k  = ()
 let lemma_InDomRestrict m ks k = ()
 
-type Equal (#key:Type) (#value:Type) (m1:t key value) (m2:t key value) =
+abstract type Equal (#key:Type) (#value:Type) (m1:t key value) (m2:t key value) =
     FEq m1.mappings m2.mappings /\ FEq m1.domain m2.domain
+
+
+abstract val lemma_equal_intro: m1:t 'key 'value -> m2:t 'key 'value ->
+                       Lemma (requires (forall k. sel m1 k = sel m2 k /\
+                                                  contains m1 k = contains m2 k))
+                       (ensures (Equal m1 m2))
+                       [SMTPatT (Equal m1 m2)]
+
+abstract val lemma_equal_elim: m1:t 'key 'value -> m2:t 'key 'value ->
+                      Lemma (requires (Equal m1 m2)) (ensures  (m1 = m2))
+                      [SMTPatT (Equal m1 m2)]
+
+abstract val lemma_equal_refl: m1:t 'key 'value -> m2:t 'key 'value ->
+                      Lemma  (requires (m1 = m2)) (ensures  (Equal m1 m2))
+		      [SMTPatT (Equal m1 m2)]
+
 
 let lemma_equal_intro m1 m2 = ()
 let lemma_equal_elim m1 m2  = ()
 let lemma_equal_refl m1 m2  = ()
 
-(* AR: this needs to be copied from .fsi, else get an error in wysteria.fst *)
-opaque type DisjointDom (#key:Type) (#value:Type) (m1:t key value) (m2:t key value) =
+let const_on (#key:Type) (#value:Type) (dom:set key) (v:value) = restrict dom (const v)
+
+type DisjointDom (#key:Type) (#value:Type) (m1:t key value) (m2:t key value) =
     (forall x.{:pattern (contains m1 x)(* ; (contains m2 x) *)} contains m1 x ==> not (contains m2 x))
+
+type HasDom (#key:Type) (#value:Type) (m:t key value) (dom:set key) =
+  (forall x. contains m x <==> mem x dom)
